530-v2

reg2nfa.thy
@@ -53,8 +53,8 @@ primrec reg2lts :: "'v regexp \<Rightarrow> 'v set\<Rightarrow>  ((('v regexp, '
     "reg2lts (LChr p) a = trans2Del1 (LChr p) a"|
     "reg2lts (r1||r2) a = trans2Del1 (r1||r2) a"|
     "reg2lts (Star r) a = trans2Del1 (Star r) a" |
-    "reg2lts (r+) a = trans2Del1 (r+) a" | 
-    "reg2lts (r?) a = trans2Del1 (r?) a" |
+    "reg2lts (Plus r) a = trans2Del1 (Plus r) a" | 
+    "reg2lts (Ques r) a = trans2Del1 (Ques r) a" |
     "reg2lts (\<epsilon>) a = trans2Del1 (\<epsilon>) a"|
     "reg2lts ESet a = trans2Del1 ESet a"|
     "reg2lts (Concat r1 r2) a = trans2Del1 (Concat r1 r2) a"
@@ -64,8 +64,8 @@ primrec reg2q :: "'v regexp \<Rightarrow> 'v set\<Rightarrow>  ('v regexp) set" 
     "reg2q (LChr p) a =  {(LChr p), \<epsilon>}"|
     "reg2q (r1||r2) a = {(r1||r2),\<epsilon>} \<union> reg2q r1 a \<union> reg2q r2 a"|
     "reg2q (Star r) a = Node_State (reg2q r a) (Star r)" |
-    "reg2q (r+) a =  Node_State (reg2q r a) (Star r) \<union> {r}" |
-    "reg2q (r?) a = {(Ques r), \<epsilon>} \<union> reg2q r a" |
+    "reg2q (Plus r) a =  Node_State (reg2q r a) (Star r) \<union> {r}" |
+    "reg2q (Ques r) a = {(Ques r), \<epsilon>} \<union> reg2q r a" |
     "reg2q ESet a = {ESet, \<epsilon>}"|
     "reg2q \<epsilon> a = {\<epsilon>}"|
     "reg2q (Concat r1 r2) a = {Concat r1 r2, r1, r2, \<epsilon>, (Concat \<epsilon> r2)}"
@@ -121,18 +121,18 @@ primrec reg2nfa :: "'v regexp \<Rightarrow> 'v set\<Rightarrow> ('v regexp,'v) N
                   \<Delta>' = snd (reg2lts (Star r) a),
                   \<I> = {(Star r)}, 
                   \<F> = {\<epsilon>}\<rparr> " |
-    "reg2nfa (r+) a= \<lparr> 
-                  \<Q> = reg2q  (r+) a,
-                  \<Sigma> = alp_reg (r+) a,
-                  \<Delta> = fst (reg2lts  (r+) a),
-                  \<Delta>' = snd (reg2lts  (r+) a),
+    "reg2nfa (Plus r) a= \<lparr> 
+                  \<Q> = reg2q  (Plus r) a,
+                  \<Sigma> = alp_reg (Plus r) a,
+                  \<Delta> = fst (reg2lts  (Plus r) a),
+                  \<Delta>' = snd (reg2lts  (Plus r) a),
                   \<I> = {(Plus r)}, 
                   \<F> = {\<epsilon>}\<rparr> " |
-    "reg2nfa (r?) a = \<lparr> 
-                  \<Q> = reg2q  (r?) a,
-                  \<Sigma> = alp_reg (r?) a,
-                  \<Delta> = fst (reg2lts  (r?) a),
-                  \<Delta>' = snd (reg2lts  (r?) a),
+    "reg2nfa (Ques r) a = \<lparr> 
+                  \<Q> = reg2q  (Ques r) a,
+                  \<Sigma> = alp_reg (Ques r) a,
+                  \<Delta> = fst (reg2lts  (Ques r) a),
+                  \<Delta>' = snd (reg2lts  (Ques r) a),
                   \<I> = {(Ques r)}, 
                   \<F> = {\<epsilon>}\<rparr> " 
 
@@ -165,7 +165,7 @@ lemma trans2Del :"fst (trans2Del1 r v) =(\<Delta> (reg2nfa r v))"
   by (simp add: transEqDel)
 
 
-lemma ll:"LTS_is_reachable ({}, {(ε, ε)}) ε [] ε"
+lemma ll:"LTS_is_reachable ({}, {(\<epsilon>, \<epsilon>)}) \<epsilon> [] \<epsilon>"
   apply auto
   done
 theorem tranl_eq :
@@ -186,7 +186,7 @@ next
       apply auto
       subgoal for w
       proof -
-        assume a1:" LTS_is_reachable ({(LChr x, {x}, ε)}, {}) ε w ε"
+        assume a1:" LTS_is_reachable ({(LChr x, {x}, \<epsilon>)}, {}) \<epsilon> w \<epsilon>"
         from a1 have "w = []" 
           by(rule LTS_is_reachable.cases)auto
         then show "w=[]" .
@@ -203,7 +203,7 @@ next
       apply auto
       subgoal for a w
       proof -
-        assume a1:"LTS_is_reachable ({(Dot, v, ε)}, {}) ε w ε"
+        assume a1:"LTS_is_reachable ({(Dot, v, \<epsilon>)}, {}) \<epsilon> w \<epsilon>"
         from a1 have "w=[]"       
           by (rule LTS_is_reachable.cases) auto
         then show "w=[]" .
@@ -211,7 +211,7 @@ next
       done
     done    
 next
-  case ε
+  case \<epsilon>
   then show ?case     
     apply (unfold \<L>_def  NFA_accept_def)
     apply auto
@@ -226,83 +226,83 @@ next
     apply auto
     subgoal for x q xa
     proof -
-      assume a1:"sem_reg r1 v = {w. ∃q∈ℐ (reg2nfa r1 v). ∃x∈ℱ (reg2nfa r1 v). LTS_is_reachable (Δ (reg2nfa r1 v), Δ' (reg2nfa r1 v)) q w x}"
-      assume a2:"sem_reg r2 v = {w. ∃q∈ℐ (reg2nfa r2 v). ∃x∈ℱ (reg2nfa r2 v). LTS_is_reachable (Δ (reg2nfa r2 v), Δ' (reg2nfa r2 v)) q w x}"
+      assume a1:"sem_reg r1 v = {w. \<exists>q\<in>\<I> (reg2nfa r1 v). \<exists>x\<in>\<F> (reg2nfa r1 v). LTS_is_reachable (\<Delta> (reg2nfa r1 v), \<Delta>' (reg2nfa r1 v)) q w x}"
+      assume a2:"sem_reg r2 v = {w. \<exists>q\<in>\<I> (reg2nfa r2 v). \<exists>x\<in>\<F> (reg2nfa r2 v). LTS_is_reachable (\<Delta> (reg2nfa r2 v), \<Delta>' (reg2nfa r2 v)) q w x}"
       assume a3:"q \<in> \<I> (reg2nfa r1 v)"
       assume a4:"xa \<in> \<F> (reg2nfa r1 v)"
-      assume a5:"LTS_is_reachable (Δ (reg2nfa r1 v), Δ' (reg2nfa r1 v)) q x xa"
-      then show "∃q''. (q'' = r1 ∨ q'' = r2 ∨ (r1 || r2, q'') ∈ snd (trans2Del1 r1 v) ∨ (r1 || r2, q'') ∈ snd (trans2Del1 r2 v)) ∧
-          LTS_is_reachable (fst (trans2Del1 r1 v) ∪ fst (trans2Del1 r2 v), insert (r1 || r2, r1) (insert (r1 || r2, r2) (snd (trans2Del1 r1 v) ∪ snd (trans2Del1 r2 v)))) q'' x ε"
+      assume a5:"LTS_is_reachable (\<Delta> (reg2nfa r1 v), \<Delta>' (reg2nfa r1 v)) q x xa"
+      then show "\<exists>q''. (q'' = r1 \<or> q'' = r2 \<or> (r1 || r2, q'') \<in> snd (trans2Del1 r1 v) \<or> (r1 || r2, q'') \<in> snd (trans2Del1 r2 v)) \<and>
+          LTS_is_reachable (fst (trans2Del1 r1 v) \<union> fst (trans2Del1 r2 v), insert (r1 || r2, r1) (insert (r1 || r2, r2) (snd (trans2Del1 r1 v) \<union> snd (trans2Del1 r2 v)))) q'' x \<epsilon>"
       proof -
          have c1:"q = r1" 
            using InitState a3 by auto
          have c2:"xa =\<epsilon>"
            using FinalState a4 by blast
-         have c3:"LTS_is_reachable (Δ (reg2nfa r1 v), Δ' (reg2nfa r1 v)) r1 x \<epsilon>"
+         have c3:"LTS_is_reachable (\<Delta> (reg2nfa r1 v), \<Delta>' (reg2nfa r1 v)) r1 x \<epsilon>"
            using a5 c1 c2 by auto
-         have c4:"LTS_is_reachable (fst (trans2Del1 r1 v), Δ' (reg2nfa r1 v)) r1 x \<epsilon>"
+         have c4:"LTS_is_reachable (fst (trans2Del1 r1 v), \<Delta>' (reg2nfa r1 v)) r1 x \<epsilon>"
            using c3 
            by (induct r1) auto
         have c5: "LTS_is_reachable (fst (trans2Del1 r1 v),snd (trans2Del1 r1 v)) r1 x \<epsilon>"
            using c4 apply (induct r1)
            by auto
-         have c6:"LTS_is_reachable (fst (trans2Del1 r1 v) ∪ fst (trans2Del1 r2 v), insert (r1 || r2, r1) (insert (r1 || r2, r2) (snd (trans2Del1 r1 v) ∪ snd (trans2Del1 r2 v)))) r1 x ε"
+         have c6:"LTS_is_reachable (fst (trans2Del1 r1 v) \<union> fst (trans2Del1 r2 v), insert (r1 || r2, r1) (insert (r1 || r2, r2) (snd (trans2Del1 r1 v) \<union> snd (trans2Del1 r2 v)))) r1 x \<epsilon>"
            using c5 
            by (metis Un_insert_right prod.collapse subLTSlemma)
-         then show "∃q''. (q'' = r1 ∨ q'' = r2 ∨ (r1 || r2, q'') ∈ snd (trans2Del1 r1 v) ∨ (r1 || r2, q'') ∈ snd (trans2Del1 r2 v)) ∧
-          LTS_is_reachable (fst (trans2Del1 r1 v) ∪ fst (trans2Del1 r2 v), insert (r1 || r2, r1) (insert (r1 || r2, r2) (snd (trans2Del1 r1 v) ∪ snd (trans2Del1 r2 v)))) q'' x ε" by auto
+         then show "\<exists>q''. (q'' = r1 \<or> q'' = r2 \<or> (r1 || r2, q'') \<in> snd (trans2Del1 r1 v) \<or> (r1 || r2, q'') \<in> snd (trans2Del1 r2 v)) \<and>
+          LTS_is_reachable (fst (trans2Del1 r1 v) \<union> fst (trans2Del1 r2 v), insert (r1 || r2, r1) (insert (r1 || r2, r2) (snd (trans2Del1 r1 v) \<union> snd (trans2Del1 r2 v)))) q'' x \<epsilon>" by auto
        qed
      qed
      subgoal for x q xa
       proof -
-      assume a1:"sem_reg r1 v = {w. ∃q∈ℐ (reg2nfa r1 v). ∃x∈ℱ (reg2nfa r1 v). LTS_is_reachable (Δ (reg2nfa r1 v), Δ' (reg2nfa r1 v)) q w x}"
-      assume a2:"sem_reg r2 v = {w. ∃q∈ℐ (reg2nfa r2 v). ∃x∈ℱ (reg2nfa r2 v). LTS_is_reachable (Δ (reg2nfa r2 v), Δ' (reg2nfa r2 v)) q w x}"
+      assume a1:"sem_reg r1 v = {w. \<exists>q\<in>\<I> (reg2nfa r1 v). \<exists>x\<in>\<F> (reg2nfa r1 v). LTS_is_reachable (\<Delta> (reg2nfa r1 v), \<Delta>' (reg2nfa r1 v)) q w x}"
+      assume a2:"sem_reg r2 v = {w. \<exists>q\<in>\<I> (reg2nfa r2 v). \<exists>x\<in>\<F> (reg2nfa r2 v). LTS_is_reachable (\<Delta> (reg2nfa r2 v), \<Delta>' (reg2nfa r2 v)) q w x}"
       assume a3:"q \<in> \<I> (reg2nfa r2 v)"
       assume a4:"xa \<in> \<F> (reg2nfa r2 v)"
-      assume a5:"LTS_is_reachable (Δ (reg2nfa r2 v), Δ' (reg2nfa r2 v)) q x xa"
-      then show " ∃q''. (q'' = r1 ∨ q'' = r2 ∨ (r1 || r2, q'') ∈ snd (trans2Del1 r1 v) ∨ (r1 || r2, q'') ∈ snd (trans2Del1 r2 v)) ∧
-          LTS_is_reachable (fst (trans2Del1 r1 v) ∪ fst (trans2Del1 r2 v), insert (r1 || r2, r1) (insert (r1 || r2, r2) (snd (trans2Del1 r1 v) ∪ snd (trans2Del1 r2 v)))) q'' x ε"
+      assume a5:"LTS_is_reachable (\<Delta> (reg2nfa r2 v), \<Delta>' (reg2nfa r2 v)) q x xa"
+      then show " \<exists>q''. (q'' = r1 \<or> q'' = r2 \<or> (r1 || r2, q'') \<in> snd (trans2Del1 r1 v) \<or> (r1 || r2, q'') \<in> snd (trans2Del1 r2 v)) \<and>
+          LTS_is_reachable (fst (trans2Del1 r1 v) \<union> fst (trans2Del1 r2 v), insert (r1 || r2, r1) (insert (r1 || r2, r2) (snd (trans2Del1 r1 v) \<union> snd (trans2Del1 r2 v)))) q'' x \<epsilon>"
       proof -
          have c1:"q = r2" 
            using InitState a3 by blast
-         have c2:"xa =ε"
+         have c2:"xa =\<epsilon>"
            using FinalState a4 by blast
-         have c3:"LTS_is_reachable (Δ (reg2nfa r2 v), Δ' (reg2nfa r2 v)) r2 x ε"
+         have c3:"LTS_is_reachable (\<Delta> (reg2nfa r2 v), \<Delta>' (reg2nfa r2 v)) r2 x \<epsilon>"
            using a5 c1 c2 by auto
-         have c4:"LTS_is_reachable (fst (trans2Del1 r2 v), Δ' (reg2nfa r2 v)) r2 x ε"
+         have c4:"LTS_is_reachable (fst (trans2Del1 r2 v), \<Delta>' (reg2nfa r2 v)) r2 x \<epsilon>"
            using c3 
            by (induct r2) auto
-        have c5: "LTS_is_reachable (fst (trans2Del1 r2 v),snd (trans2Del1 r2 v)) r2 x ε"
+        have c5: "LTS_is_reachable (fst (trans2Del1 r2 v),snd (trans2Del1 r2 v)) r2 x \<epsilon>"
            using c4 apply (induct r2)
            by auto
-        have c6:"LTS_is_reachable (fst (trans2Del1 r1 v) ∪ fst (trans2Del1 r2 v), insert (r1 || r2, r1) (insert (r1 || r2, r2) (snd (trans2Del1 r1 v) ∪ snd (trans2Del1 r2 v)))) r2 x ε"
+        have c6:"LTS_is_reachable (fst (trans2Del1 r1 v) \<union> fst (trans2Del1 r2 v), insert (r1 || r2, r1) (insert (r1 || r2, r2) (snd (trans2Del1 r1 v) \<union> snd (trans2Del1 r2 v)))) r2 x \<epsilon>"
           using c5 
           by (smt (z3) Un_insert_left subLTSlemma sup_commute surjective_pairing)
-         then show " ∃q''. (q'' = r1 ∨ q'' = r2 ∨ (r1 || r2, q'') ∈ snd (trans2Del1 r1 v) ∨ (r1 || r2, q'') ∈ snd (trans2Del1 r2 v)) ∧
-          LTS_is_reachable (fst (trans2Del1 r1 v) ∪ fst (trans2Del1 r2 v), insert (r1 || r2, r1) (insert (r1 || r2, r2) (snd (trans2Del1 r1 v) ∪ snd (trans2Del1 r2 v)))) q'' x ε" by auto
+         then show " \<exists>q''. (q'' = r1 \<or> q'' = r2 \<or> (r1 || r2, q'') \<in> snd (trans2Del1 r1 v) \<or> (r1 || r2, q'') \<in> snd (trans2Del1 r2 v)) \<and>
+          LTS_is_reachable (fst (trans2Del1 r1 v) \<union> fst (trans2Del1 r2 v), insert (r1 || r2, r1) (insert (r1 || r2, r2) (snd (trans2Del1 r1 v) \<union> snd (trans2Del1 r2 v)))) q'' x \<epsilon>" by auto
        qed
      qed
      subgoal for x
      proof -
-       assume a1:"sem_reg r1 v = {w. ∃q∈ℐ (reg2nfa r1 v). ∃x∈ℱ (reg2nfa r1 v). LTS_is_reachable (Δ (reg2nfa r1 v), Δ' (reg2nfa r1 v)) q w x}" 
-       assume a2:"sem_reg r2 v = {w. ∃q∈ℐ (reg2nfa r2 v). ∃x∈ℱ (reg2nfa r2 v). LTS_is_reachable (Δ (reg2nfa r2 v), Δ' (reg2nfa r2 v)) q w x}"
-       assume a3:"LTS_is_reachable (fst (trans2Del1 r1 v) ∪ fst (trans2Del1 r2 v), insert (r1 || r2, r1) (insert (r1 || r2, r2) (snd (trans2Del1 r1 v) ∪ snd (trans2Del1 r2 v)))) (r1 || r2) x ε"
-       assume a4:"∀q∈ℐ (reg2nfa r2 v). ∀xa∈ℱ (reg2nfa r2 v). ¬ LTS_is_reachable (Δ (reg2nfa r2 v), Δ' (reg2nfa r2 v)) q x xa"
-       show "∃q∈ℐ (reg2nfa r1 v). ∃xa∈ℱ (reg2nfa r1 v). LTS_is_reachable (Δ (reg2nfa r1 v), Δ' (reg2nfa r1 v)) q x xa" 
+       assume a1:"sem_reg r1 v = {w. \<exists>q\<in>\<I> (reg2nfa r1 v). \<exists>x\<in>\<F> (reg2nfa r1 v). LTS_is_reachable (\<Delta> (reg2nfa r1 v), \<Delta>' (reg2nfa r1 v)) q w x}" 
+       assume a2:"sem_reg r2 v = {w. \<exists>q\<in>\<I> (reg2nfa r2 v). \<exists>x\<in>\<F> (reg2nfa r2 v). LTS_is_reachable (\<Delta> (reg2nfa r2 v), \<Delta>' (reg2nfa r2 v)) q w x}"
+       assume a3:"LTS_is_reachable (fst (trans2Del1 r1 v) \<union> fst (trans2Del1 r2 v), insert (r1 || r2, r1) (insert (r1 || r2, r2) (snd (trans2Del1 r1 v) \<union> snd (trans2Del1 r2 v)))) (r1 || r2) x \<epsilon>"
+       assume a4:"\<forall>q\<in>\<I> (reg2nfa r2 v). \<forall>xa\<in>\<F> (reg2nfa r2 v). \<not> LTS_is_reachable (\<Delta> (reg2nfa r2 v), \<Delta>' (reg2nfa r2 v)) q x xa"
+       show "\<exists>q\<in>\<I> (reg2nfa r1 v). \<exists>xa\<in>\<F> (reg2nfa r1 v). LTS_is_reachable (\<Delta> (reg2nfa r1 v), \<Delta>' (reg2nfa r1 v)) q x xa" 
        proof -
-         have c1:" ¬ LTS_is_reachable (Δ (reg2nfa r2 v), Δ' (reg2nfa r2 v)) r2 x ε" using a4 
+         have c1:" \<not> LTS_is_reachable (\<Delta> (reg2nfa r2 v), \<Delta>' (reg2nfa r2 v)) r2 x \<epsilon>" using a4 
            using finalSet
            by (simp add: finalSet initalSet)
-        have c2:" ¬ LTS_is_reachable (fst (trans2Del1 r2 v), (snd (trans2Del1 r2 v))) r2 x ε" using c1 
+        have c2:" \<not> LTS_is_reachable (fst (trans2Del1 r2 v), (snd (trans2Del1 r2 v))) r2 x \<epsilon>" using c1 
           by (induct r2) auto
-        have c3:" ¬ LTS_is_reachable (fst (trans2Del1 r2 v), insert (r1 || r2, r2) (snd (trans2Del1 r2 v))) (r1||r2) x ε" using c2
+        have c3:" \<not> LTS_is_reachable (fst (trans2Del1 r2 v), insert (r1 || r2, r2) (snd (trans2Del1 r2 v))) (r1||r2) x \<epsilon>" using c2
           apply simp
           apply(rule LTS_is_reachable.induct)
              apply auto
           sorry
-         have c4:"LTS_is_reachable (fst (trans2Del1 r1 v) ∪ fst (trans2Del1 r2 v), insert (r1 || r2, r1) (insert (r1 || r2, r2) (snd (trans2Del1 r1 v) ∪ snd (trans2Del1 r2 v)))) (r1 || r2) [] r1"
+         have c4:"LTS_is_reachable (fst (trans2Del1 r1 v) \<union> fst (trans2Del1 r2 v), insert (r1 || r2, r1) (insert (r1 || r2, r2) (snd (trans2Del1 r1 v) \<union> snd (trans2Del1 r2 v)))) (r1 || r2) [] r1"
            by auto
-         have c5:"LTS_is_reachable (fst (trans2Del1 r1 v) ∪ fst (trans2Del1 r2 v), insert (r1 || r2, r1) (insert (r1 || r2, r2) (snd (trans2Del1 r1 v) ∪ snd (trans2Del1 r2 v)))) (r1 || r2) [] r2"
+         have c5:"LTS_is_reachable (fst (trans2Del1 r1 v) \<union> fst (trans2Del1 r2 v), insert (r1 || r2, r1) (insert (r1 || r2, r2) (snd (trans2Del1 r1 v) \<union> snd (trans2Del1 r2 v)))) (r1 || r2) [] r2"
            by auto
          then show ?thesis sorry
        qed
@@ -315,93 +315,93 @@ next
     apply auto
     subgoal for a b q xa qa xb 
     proof -
-    assume a1:"sem_reg r1 v ={w. ∃q∈ℐ (reg2nfa r1 v). ∃x∈ℱ (reg2nfa r1 v). LTS_is_reachable (Δ (reg2nfa r1 v), Δ' (reg2nfa r1 v)) q w x}"
-    assume a2:"sem_reg r2 v ={w. ∃q∈ℐ (reg2nfa r2 v). ∃x∈ℱ (reg2nfa r2 v). LTS_is_reachable (Δ (reg2nfa r2 v), Δ' (reg2nfa r2 v)) q w x}"
+    assume a1:"sem_reg r1 v ={w. \<exists>q\<in>\<I> (reg2nfa r1 v). \<exists>x\<in>\<F> (reg2nfa r1 v). LTS_is_reachable (\<Delta> (reg2nfa r1 v), \<Delta>' (reg2nfa r1 v)) q w x}"
+    assume a2:"sem_reg r2 v ={w. \<exists>q\<in>\<I> (reg2nfa r2 v). \<exists>x\<in>\<F> (reg2nfa r2 v). LTS_is_reachable (\<Delta> (reg2nfa r2 v), \<Delta>' (reg2nfa r2 v)) q w x}"
     assume a3:"q \<in> \<I> (reg2nfa r1 v)"
     assume a4:"xa \<in> \<F> (reg2nfa r1 v)"
-    assume a5:"LTS_is_reachable (Δ (reg2nfa r1 v), Δ' (reg2nfa r1 v)) q a xa"
+    assume a5:"LTS_is_reachable (\<Delta> (reg2nfa r1 v), \<Delta>' (reg2nfa r1 v)) q a xa"
     assume a6:"qa \<in> \<I> (reg2nfa r2 v)"
     assume a7:"xb \<in> \<F> (reg2nfa r2 v)"
-    assume a8:"LTS_is_reachable (Δ (reg2nfa r2 v), Δ' (reg2nfa r2 v)) qa b xb"
+    assume a8:"LTS_is_reachable (\<Delta> (reg2nfa r2 v), \<Delta>' (reg2nfa r2 v)) qa b xb"
     from a3 have c1:"q = r1" 
       using InitState by blast
-    from a4 have c2:"xa = ε" 
+    from a4 have c2:"xa = \<epsilon>" 
       using FinalState by blast
-    from c1 c2 a5 have c3:"LTS_is_reachable (Δ (reg2nfa r1 v), Δ' (reg2nfa r1 v)) r1 a ε" 
+    from c1 c2 a5 have c3:"LTS_is_reachable (\<Delta> (reg2nfa r1 v), \<Delta>' (reg2nfa r1 v)) r1 a \<epsilon>" 
       by auto
     from a6 have c4: "qa = r2" 
       using InitState by blast
-    from a7 have c5: "xb = ε"
+    from a7 have c5: "xb = \<epsilon>"
       using FinalState by blast 
-    from c4 c5 a8 have c6: "LTS_is_reachable (Δ (reg2nfa r2 v), Δ' (reg2nfa r2 v)) r2 b ε" 
+    from c4 c5 a8 have c6: "LTS_is_reachable (\<Delta> (reg2nfa r2 v), \<Delta>' (reg2nfa r2 v)) r2 b \<epsilon>" 
       by auto
-    from c3 c6 have c7:"LTS_is_reachable (Δ (reg2nfa (Concat r1 r2) v), Δ' (reg2nfa (Concat r1 r2) v))  (Concat r1 r2) (a @ b) ε" 
+    from c3 c6 have c7:"LTS_is_reachable (\<Delta> (reg2nfa (Concat r1 r2) v), \<Delta>' (reg2nfa (Concat r1 r2) v))  (Concat r1 r2) (a @ b) \<epsilon>" 
       proof -
-      assume b1:"LTS_is_reachable (Δ (reg2nfa r1 v), Δ' (reg2nfa r1 v)) r1 a ε"
-      assume b2:"LTS_is_reachable (Δ (reg2nfa r2 v), Δ' (reg2nfa r2 v)) r2 b ε"
-      have e1:"LTS_is_reachable (fst (trans2Del1 r1 v), snd (trans2Del1 r1 v)) r1 a ε" 
+      assume b1:"LTS_is_reachable (\<Delta> (reg2nfa r1 v), \<Delta>' (reg2nfa r1 v)) r1 a \<epsilon>"
+      assume b2:"LTS_is_reachable (\<Delta> (reg2nfa r2 v), \<Delta>' (reg2nfa r2 v)) r2 b \<epsilon>"
+      have e1:"LTS_is_reachable (fst (trans2Del1 r1 v), snd (trans2Del1 r1 v)) r1 a \<epsilon>" 
         using b1 by (induct r1)  auto
-      have e2:"LTS_is_reachable (fst (trans2Del1 r2 v), snd (trans2Del1 r2 v)) r2 b ε" 
+      have e2:"LTS_is_reachable (fst (trans2Del1 r2 v), snd (trans2Del1 r2 v)) r2 b \<epsilon>" 
         using b2 by (induct r2)  auto
-      from b1 have e3:"LTS_is_reachable (Δ (reg2nfa (Concat r1 r2) v), Δ' (reg2nfa (Concat r1 r2) v)) (Concat r1 r2) a r2"
+      from b1 have e3:"LTS_is_reachable (\<Delta> (reg2nfa (Concat r1 r2) v), \<Delta>' (reg2nfa (Concat r1 r2) v)) (Concat r1 r2) a r2"
         apply simp
         proof - 
-          assume a1:"LTS_is_reachable (Δ (reg2nfa r1 v), Δ' (reg2nfa r1 v)) r1 a ε"
-          have c1:"LTS_is_reachable (fst (trans2Del1 r1 v), snd (trans2Del1 r1 v)) r1 a ε"
+          assume a1:"LTS_is_reachable (\<Delta> (reg2nfa r1 v), \<Delta>' (reg2nfa r1 v)) r1 a \<epsilon>"
+          have c1:"LTS_is_reachable (fst (trans2Del1 r1 v), snd (trans2Del1 r1 v)) r1 a \<epsilon>"
             using a1 by (induct r1) auto
-          have c2:"LTS_is_reachable (fst (trans2Del1 r1 v) ∪ fst (trans2Del1 r2 v),snd (trans2Del1 r1 v) \<union> snd (trans2Del1 r2 v)) r1 a   ε"
+          have c2:"LTS_is_reachable (fst (trans2Del1 r1 v) \<union> fst (trans2Del1 r2 v),snd (trans2Del1 r1 v) \<union> snd (trans2Del1 r2 v)) r1 a   \<epsilon>"
             using c1 by auto
           have c3:"LTS_is_reachable
-           ({(Concat q r2, va, Concat q' r2) |q va q'. (q, va, q') ∈ fst (trans2Del1 r1 v)} ∪ fst (trans2Del1 r2 v),
-            insert (Concat ε r2, r2) ({(Concat q r2, Concat q' r2) |q q'. (q, q') ∈ snd (trans2Del1 r1 v)} ∪ snd (trans2Del1 r2 v)))
-           (Concat r1 r2) a (Concat ε r2)"
+           ({(Concat q r2, va, Concat q' r2) |q va q'. (q, va, q') \<in> fst (trans2Del1 r1 v)} \<union> fst (trans2Del1 r2 v),
+            insert (Concat \<epsilon> r2, r2) ({(Concat q r2, Concat q' r2) |q q'. (q, q') \<in> snd (trans2Del1 r1 v)} \<union> snd (trans2Del1 r2 v)))
+           (Concat r1 r2) a (Concat \<epsilon> r2)"
             using c1 apply simp    
             apply (induction rule: LTS_is_reachable.induct)
             by auto+
            have c4:"LTS_is_reachable
-           ({(Concat q r2, va, Concat q' r2) |q va q'. (q, va, q') ∈ fst (trans2Del1 r1 v)} ∪ fst (trans2Del1 r2 v),
-            insert (Concat ε r2, r2) ({(Concat q r2, Concat q' r2) |q q'. (q, q') ∈ snd (trans2Del1 r1 v)} ∪ snd (trans2Del1 r2 v)))
-           (Concat ε r2) [] r2"
+           ({(Concat q r2, va, Concat q' r2) |q va q'. (q, va, q') \<in> fst (trans2Del1 r1 v)} \<union> fst (trans2Del1 r2 v),
+            insert (Concat \<epsilon> r2, r2) ({(Concat q r2, Concat q' r2) |q q'. (q, q') \<in> snd (trans2Del1 r1 v)} \<union> snd (trans2Del1 r2 v)))
+           (Concat \<epsilon> r2) [] r2"
              using c3 by auto 
            have c5:"LTS_is_reachable
-           ({(Concat q r2, va, Concat q' r2) |q va q'. (q, va, q') ∈ fst (trans2Del1 r1 v)} ∪ fst (trans2Del1 r2 v),
-            insert (Concat ε r2, r2) ({(Concat q r2, Concat q' r2) |q q'. (q, q') ∈ snd (trans2Del1 r1 v)} ∪ snd (trans2Del1 r2 v)))
+           ({(Concat q r2, va, Concat q' r2) |q va q'. (q, va, q') \<in> fst (trans2Del1 r1 v)} \<union> fst (trans2Del1 r2 v),
+            insert (Concat \<epsilon> r2, r2) ({(Concat q r2, Concat q' r2) |q q'. (q, q') \<in> snd (trans2Del1 r1 v)} \<union> snd (trans2Del1 r2 v)))
            (Concat r1 r2) a r2"
              using c3 c4 
              by (induction rule: LTS_is_reachable.induct) auto
-            then show "LTS_is_reachable ({(Concat q r2, va, Concat q' r2) |q va q'. (q, va, q') ∈ fst (trans2Del1 r1 v)} ∪ fst (trans2Del1 r2 v),
-          insert (Concat ε r2, r2) ({(Concat q r2, Concat q' r2) |q q'. (q, q') ∈ snd (trans2Del1 r1 v)} ∪ snd (trans2Del1 r2 v)))
+            then show "LTS_is_reachable ({(Concat q r2, va, Concat q' r2) |q va q'. (q, va, q') \<in> fst (trans2Del1 r1 v)} \<union> fst (trans2Del1 r2 v),
+          insert (Concat \<epsilon> r2, r2) ({(Concat q r2, Concat q' r2) |q q'. (q, q') \<in> snd (trans2Del1 r1 v)} \<union> snd (trans2Del1 r2 v)))
          (Concat r1 r2) a  r2"  
               by blast
           qed
-      have e4:"LTS_is_reachable (Δ (reg2nfa (Concat r1 r2) v), Δ' (reg2nfa (Concat r1 r2) v)) r2 b ε"
+      have e4:"LTS_is_reachable (\<Delta> (reg2nfa (Concat r1 r2) v), \<Delta>' (reg2nfa (Concat r1 r2) v)) r2 b \<epsilon>"
         using e2 apply simp
         by (smt (z3) Un_commute Un_insert_right subLTSlemma)
-      show " LTS_is_reachable (Δ (reg2nfa (Concat r1 r2) v), Δ' (reg2nfa (Concat r1 r2) v)) (Concat r1 r2) (a @ b) ε" 
+      show " LTS_is_reachable (\<Delta> (reg2nfa (Concat r1 r2) v), \<Delta>' (reg2nfa (Concat r1 r2) v)) (Concat r1 r2) (a @ b) \<epsilon>" 
         by (meson e3 e4 joinLTSlemma)
     qed
-    have e1:"LTS_is_reachable (Δ (reg2nfa ε v), Δ' (reg2nfa ε v)) ε [] ε"
+    have e1:"LTS_is_reachable (\<Delta> (reg2nfa \<epsilon> v), \<Delta>' (reg2nfa \<epsilon> v)) \<epsilon> [] \<epsilon>"
       by auto
-    have e2:"LTS_is_reachable (fst (trans2Del1 r2 v), snd (trans2Del1 r2 v))  r2 b ε"
+    have e2:"LTS_is_reachable (fst (trans2Del1 r2 v), snd (trans2Del1 r2 v))  r2 b \<epsilon>"
       using c6 by (induct r2) auto
     have e3:"LTS_is_reachable
-           ({(Concat q r2, va, Concat q' r2) |q va q'. (q, va, q') ∈ fst (trans2Del1 r1 v)} ∪ fst (trans2Del1 r2 v),
-           ({(Concat q r2, Concat q' r2) |q q'. (q, q') ∈ snd (trans2Del1 r1 v)} ∪ snd (trans2Del1 r2 v)))
-           r2 b ε"
+           ({(Concat q r2, va, Concat q' r2) |q va q'. (q, va, q') \<in> fst (trans2Del1 r1 v)} \<union> fst (trans2Del1 r2 v),
+           ({(Concat q r2, Concat q' r2) |q q'. (q, q') \<in> snd (trans2Del1 r1 v)} \<union> snd (trans2Del1 r2 v)))
+           r2 b \<epsilon>"
       using e2 
       apply simp
       by (simp add: sup.commute)
     have e4:"LTS_is_reachable
-           ({(Concat q r2, va, Concat q' r2) |q va q'. (q, va, q') ∈ fst (trans2Del1 ε v)} ∪ fst (trans2Del1 r2 v),
-           insert (Concat ε r2, r2) ({(Concat q r2, Concat q' r2) |q q'. (q, q') ∈ snd (trans2Del1 ε v)} ∪ snd (trans2Del1 r2 v)))
-           r2 ([]@b) ε"
+           ({(Concat q r2, va, Concat q' r2) |q va q'. (q, va, q') \<in> fst (trans2Del1 \<epsilon> v)} \<union> fst (trans2Del1 r2 v),
+           insert (Concat \<epsilon> r2, r2) ({(Concat q r2, Concat q' r2) |q q'. (q, q') \<in> snd (trans2Del1 \<epsilon> v)} \<union> snd (trans2Del1 r2 v)))
+           r2 ([]@b) \<epsilon>"
       using e3 
       by (metis (no_types, lifting) Un_commute Un_insert_right append_self_conv2 e2 prod.collapse subLTSlemma)
-    show "∃q''. (r1 = ε ∧ q'' = r2 ∨ (∃q'. q'' = Concat q' r2 ∧ (r1, q') ∈ snd (trans2Del1 r1 v)) ∨ (Concat r1 r2, q'') ∈ snd (trans2Del1 r2 v)) ∧
+    show "\<exists>q''. (r1 = \<epsilon> \<and> q'' = r2 \<or> (\<exists>q'. q'' = Concat q' r2 \<and> (r1, q') \<in> snd (trans2Del1 r1 v)) \<or> (Concat r1 r2, q'') \<in> snd (trans2Del1 r2 v)) \<and>
           LTS_is_reachable
-           ({(Concat q r2, va, Concat q' r2) |q va q'. (q, va, q') ∈ fst (trans2Del1 r1 v)} ∪ fst (trans2Del1 r2 v),
-            insert (Concat ε r2, r2) ({(Concat q r2, Concat q' r2) |q q'. (q, q') ∈ snd (trans2Del1 r1 v)} ∪ snd (trans2Del1 r2 v)))
-           q'' (a @ b) ε"
+           ({(Concat q r2, va, Concat q' r2) |q va q'. (q, va, q') \<in> fst (trans2Del1 r1 v)} \<union> fst (trans2Del1 r2 v),
+            insert (Concat \<epsilon> r2, r2) ({(Concat q r2, Concat q' r2) |q q'. (q, q') \<in> snd (trans2Del1 r1 v)} \<union> snd (trans2Del1 r2 v)))
+           q'' (a @ b) \<epsilon>"
       sorry
   qed
   subgoal for x 
@@ -414,16 +414,16 @@ next
      apply auto 
     subgoal for x 
     proof -
-      assume a1:"sem_reg r v = {w. ∃q∈ℐ (reg2nfa r v). ∃x∈ℱ (reg2nfa r v). LTS_is_reachable (Δ (reg2nfa r v), Δ' (reg2nfa r v)) q w x}"
-      assume a2:"x ∈ star {w. ∃q∈ℐ (reg2nfa r v). ∃x∈ℱ (reg2nfa r v). LTS_is_reachable (Δ (reg2nfa r v), Δ' (reg2nfa r v)) q w x}"
-      show "∃q''. (q'' = ε ∨ (Star r, q'') ∈ Delta2_State (insert (Star r, r) (snd (trans2Del1 r v))) (Star r)) ∧
-          LTS_is_reachable (Delta1_State (fst (trans2Del1 r v)) r, insert (Star r, ε) (Delta2_State (insert (Star r, r) (snd (trans2Del1 r v))) (Star r))) q'' x ε" sorry
+      assume a1:"sem_reg r v = {w. \<exists>q\<in>\<I> (reg2nfa r v). \<exists>x\<in>\<F> (reg2nfa r v). LTS_is_reachable (\<Delta> (reg2nfa r v), \<Delta>' (reg2nfa r v)) q w x}"
+      assume a2:"x \<in> star {w. \<exists>q\<in>\<I> (reg2nfa r v). \<exists>x\<in>\<F> (reg2nfa r v). LTS_is_reachable (\<Delta> (reg2nfa r v), \<Delta>' (reg2nfa r v)) q w x}"
+      show "\<exists>q''. (q'' = \<epsilon> \<or> (Star r, q'') \<in> Delta2_State (insert (Star r, r) (snd (trans2Del1 r v))) (Star r)) \<and>
+          LTS_is_reachable (Delta1_State (fst (trans2Del1 r v)) r, insert (Star r, \<epsilon>) (Delta2_State (insert (Star r, r) (snd (trans2Del1 r v))) (Star r))) q'' x \<epsilon>" sorry
     qed
     subgoal for x 
     proof - 
-      assume a1:"sem_reg r v = {w. ∃q∈ℐ (reg2nfa r v). ∃x∈ℱ (reg2nfa r v). LTS_is_reachable (Δ (reg2nfa r v), Δ' (reg2nfa r v)) q w x}"
-      assume a2:"LTS_is_reachable (Delta1_State (fst (trans2Del1 r v)) r, insert (Star r, ε) (Delta2_State (insert (Star r, r) (snd (trans2Del1 r v))) (Star r))) (Star r) x ε"
-      show "x ∈ star {w. ∃q∈ℐ (reg2nfa r v). ∃x∈ℱ (reg2nfa r v). LTS_is_reachable (Δ (reg2nfa r v), Δ' (reg2nfa r v)) q w x}"
+      assume a1:"sem_reg r v = {w. \<exists>q\<in>\<I> (reg2nfa r v). \<exists>x\<in>\<F> (reg2nfa r v). LTS_is_reachable (\<Delta> (reg2nfa r v), \<Delta>' (reg2nfa r v)) q w x}"
+      assume a2:"LTS_is_reachable (Delta1_State (fst (trans2Del1 r v)) r, insert (Star r, \<epsilon>) (Delta2_State (insert (Star r, r) (snd (trans2Del1 r v))) (Star r))) (Star r) x \<epsilon>"
+      show "x \<in> star {w. \<exists>q\<in>\<I> (reg2nfa r v). \<exists>x\<in>\<F> (reg2nfa r v). LTS_is_reachable (\<Delta> (reg2nfa r v), \<Delta>' (reg2nfa r v)) q w x}"
         sorry
     qed
     done
@@ -434,57 +434,57 @@ next
     apply auto 
     subgoal for x q xa 
     proof -
-      assume a1:"sem_reg r v = {w. ∃q∈ℐ (reg2nfa r v). ∃x∈ℱ (reg2nfa r v). LTS_is_reachable (Δ (reg2nfa r v), Δ' (reg2nfa r v)) q w x}"
-      assume a2:"q ∈ ℐ (reg2nfa r v)"
-      assume a3:"xa ∈ ℱ (reg2nfa r v)"
-      assume a4:"LTS_is_reachable (Δ (reg2nfa r v), Δ' (reg2nfa r v)) q x xa"
-      show " ∃q''. (r+, q'')
-          ∈ Delta2_State
-              (insert (r+, Concat r (Star r))
-                (insert (Concat r (Star r), r) (insert (Star r, r) ({(Concat q (Star r), Concat q' (Star r)) |q q'. (q, q') ∈ snd (trans2Del1 r v)} ∪ snd (trans2Del1 r v)))))
-              (Star r) ∧
+      assume a1:"sem_reg r v = {w. \<exists>q\<in>\<I> (reg2nfa r v). \<exists>x\<in>\<F> (reg2nfa r v). LTS_is_reachable (\<Delta> (reg2nfa r v), \<Delta>' (reg2nfa r v)) q w x}"
+      assume a2:"q \<in> \<I> (reg2nfa r v)"
+      assume a3:"xa \<in> \<F> (reg2nfa r v)"
+      assume a4:"LTS_is_reachable (\<Delta> (reg2nfa r v), \<Delta>' (reg2nfa r v)) q x xa"
+      show " \<exists>q''. ( Plus r, q'')
+          \<in> Delta2_State
+              (insert ( Plus r, Concat r (Star r))
+                (insert (Concat r (Star r), r) (insert (Star r, r) ({(Concat q (Star r), Concat q' (Star r)) |q q'. (q, q') \<in> snd (trans2Del1 r v)} \<union> snd (trans2Del1 r v)))))
+              (Star r) \<and>
           LTS_is_reachable
-           (Delta1_State ({(Concat q (Star r), va, Concat q' (Star r)) |q va q'. (q, va, q') ∈ fst (trans2Del1 r v)} ∪ Delta1_State (fst (trans2Del1 r v)) r) r,
-            insert (Star r, ε)
+           (Delta1_State ({(Concat q (Star r), va, Concat q' (Star r)) |q va q'. (q, va, q') \<in> fst (trans2Del1 r v)} \<union> Delta1_State (fst (trans2Del1 r v)) r) r,
+            insert (Star r, \<epsilon>)
              (Delta2_State
-               (insert (r+, Concat r (Star r))
-                 (insert (Concat r (Star r), r) (insert (Star r, r) ({(Concat q (Star r), Concat q' (Star r)) |q q'. (q, q') ∈ snd (trans2Del1 r v)} ∪ snd (trans2Del1 r v)))))
+               (insert ( Plus r, Concat r (Star r))
+                 (insert (Concat r (Star r), r) (insert (Star r, r) ({(Concat q (Star r), Concat q' (Star r)) |q q'. (q, q') \<in> snd (trans2Del1 r v)} \<union> snd (trans2Del1 r v)))))
                (Star r)))
-           q'' x ε" 
+           q'' x \<epsilon>" 
         sorry 
     qed
     subgoal for x 
     proof -
-      assume a1:"sem_reg r v = {w. ∃q∈ℐ (reg2nfa r v). ∃x∈ℱ (reg2nfa r v). LTS_is_reachable (Δ (reg2nfa r v), Δ' (reg2nfa r v)) q w x}"
-      assume a2:"x ∈ star {w. ∃q∈ℐ (reg2nfa r v). ∃x∈ℱ (reg2nfa r v). LTS_is_reachable (Δ (reg2nfa r v), Δ' (reg2nfa r v)) q w x}"
-      show "∃q''. (r+, q'')
-            ∈ Delta2_State
-                (insert (r+, Concat r (Star r))
-                  (insert (Concat r (Star r), r) (insert (Star r, r) ({(Concat q (Star r), Concat q' (Star r)) |q q'. (q, q') ∈ snd (trans2Del1 r v)} ∪ snd (trans2Del1 r v)))))
-                (Star r) ∧
+      assume a1:"sem_reg r v = {w. \<exists>q\<in>\<I> (reg2nfa r v). \<exists>x\<in>\<F> (reg2nfa r v). LTS_is_reachable (\<Delta> (reg2nfa r v), \<Delta>' (reg2nfa r v)) q w x}"
+      assume a2:"x \<in> star {w. \<exists>q\<in>\<I> (reg2nfa r v). \<exists>x\<in>\<F> (reg2nfa r v). LTS_is_reachable (\<Delta> (reg2nfa r v), \<Delta>' (reg2nfa r v)) q w x}"
+      show "\<exists>q''. ( Plus r, q'')
+            \<in> Delta2_State
+                (insert ( Plus r, Concat r (Star r))
+                  (insert (Concat r (Star r), r) (insert (Star r, r) ({(Concat q (Star r), Concat q' (Star r)) |q q'. (q, q') \<in> snd (trans2Del1 r v)} \<union> snd (trans2Del1 r v)))))
+                (Star r) \<and>
             LTS_is_reachable
-             (Delta1_State ({(Concat q (Star r), va, Concat q' (Star r)) |q va q'. (q, va, q') ∈ fst (trans2Del1 r v)} ∪ Delta1_State (fst (trans2Del1 r v)) r) r,
-              insert (Star r, ε)
+             (Delta1_State ({(Concat q (Star r), va, Concat q' (Star r)) |q va q'. (q, va, q') \<in> fst (trans2Del1 r v)} \<union> Delta1_State (fst (trans2Del1 r v)) r) r,
+              insert (Star r, \<epsilon>)
                (Delta2_State
-                 (insert (r+, Concat r (Star r))
-                   (insert (Concat r (Star r), r) (insert (Star r, r) ({(Concat q (Star r), Concat q' (Star r)) |q q'. (q, q') ∈ snd (trans2Del1 r v)} ∪ snd (trans2Del1 r v)))))
+                 (insert ( Plus r, Concat r (Star r))
+                   (insert (Concat r (Star r), r) (insert (Star r, r) ({(Concat q (Star r), Concat q' (Star r)) |q q'. (q, q') \<in> snd (trans2Del1 r v)} \<union> snd (trans2Del1 r v)))))
                  (Star r)))
-             q'' x ε"
+             q'' x \<epsilon>"
         sorry
     qed
     subgoal for x 
     proof -
-      assume a1:"sem_reg r v = {w. ∃q∈ℐ (reg2nfa r v). ∃x∈ℱ (reg2nfa r v). LTS_is_reachable (Δ (reg2nfa r v), Δ' (reg2nfa r v)) q w x}"
-      assume a2:"x ∉ star {w. ∃q∈ℐ (reg2nfa r v). ∃x∈ℱ (reg2nfa r v). LTS_is_reachable (Δ (reg2nfa r v), Δ' (reg2nfa r v)) q w x}"
+      assume a1:"sem_reg r v = {w. \<exists>q\<in>\<I> (reg2nfa r v). \<exists>x\<in>\<F> (reg2nfa r v). LTS_is_reachable (\<Delta> (reg2nfa r v), \<Delta>' (reg2nfa r v)) q w x}"
+      assume a2:"x \<notin> star {w. \<exists>q\<in>\<I> (reg2nfa r v). \<exists>x\<in>\<F> (reg2nfa r v). LTS_is_reachable (\<Delta> (reg2nfa r v), \<Delta>' (reg2nfa r v)) q w x}"
       assume a3:"LTS_is_reachable
-     (Delta1_State ({(Concat q (Star r), va, Concat q' (Star r)) |q va q'. (q, va, q') ∈ fst (trans2Del1 r v)} ∪ Delta1_State (fst (trans2Del1 r v)) r) r,
-      insert (Star r, ε)
+     (Delta1_State ({(Concat q (Star r), va, Concat q' (Star r)) |q va q'. (q, va, q') \<in> fst (trans2Del1 r v)} \<union> Delta1_State (fst (trans2Del1 r v)) r) r,
+      insert (Star r, \<epsilon>)
        (Delta2_State
-         (insert (r+, Concat r (Star r))
-           (insert (Concat r (Star r), r) (insert (Star r, r) ({(Concat q (Star r), Concat q' (Star r)) |q q'. (q, q') ∈ snd (trans2Del1 r v)} ∪ snd (trans2Del1 r v)))))
+         (insert ( Plus r, Concat r (Star r))
+           (insert (Concat r (Star r), r) (insert (Star r, r) ({(Concat q (Star r), Concat q' (Star r)) |q q'. (q, q') \<in> snd (trans2Del1 r v)} \<union> snd (trans2Del1 r v)))))
          (Star r)))
-     r+ x ε"
-      show "    ∃q∈ℐ (reg2nfa r v). ∃xa∈ℱ (reg2nfa r v). LTS_is_reachable (Δ (reg2nfa r v), Δ' (reg2nfa r v)) q x xa"
+      (Plus r) x \<epsilon>"
+      show "    \<exists>q\<in>\<I> (reg2nfa r v). \<exists>xa\<in>\<F> (reg2nfa r v). LTS_is_reachable (\<Delta> (reg2nfa r v), \<Delta>' (reg2nfa r v)) q x xa"
         sorry
     qed
     done
@@ -495,20 +495,20 @@ next
     apply auto 
     subgoal for x q xa 
     proof -
-      assume a1:"sem_reg r v = {w. ∃q∈ℐ (reg2nfa r v). ∃x∈ℱ (reg2nfa r v). LTS_is_reachable (Δ (reg2nfa r v), Δ' (reg2nfa r v)) q w x}"
-      assume a2:"sem_reg r v = {w. ∃q∈ℐ (reg2nfa r v). ∃x∈ℱ (reg2nfa r v). LTS_is_reachable (Δ (reg2nfa r v), Δ' (reg2nfa r v)) q w x}"
-      assume a3:"q ∈ ℐ (reg2nfa r v)"
-      assume a4:" xa ∈ ℱ (reg2nfa r v)"
-      assume a5:"LTS_is_reachable (Δ (reg2nfa r v), Δ' (reg2nfa r v)) q x xa"
-      show "∃q''. (q'' = ε ∨ q'' = r ∨ (r?, q'') ∈ snd (trans2Del1 r v)) ∧ LTS_is_reachable (fst (trans2Del1 r v), insert (r?, ε) (insert (r?, r) (snd (trans2Del1 r v)))) q'' x ε"
+      assume a1:"sem_reg r v = {w. \<exists>q\<in>\<I> (reg2nfa r v). \<exists>x\<in>\<F> (reg2nfa r v). LTS_is_reachable (\<Delta> (reg2nfa r v), \<Delta>' (reg2nfa r v)) q w x}"
+      assume a2:"sem_reg r v = {w. \<exists>q\<in>\<I> (reg2nfa r v). \<exists>x\<in>\<F> (reg2nfa r v). LTS_is_reachable (\<Delta> (reg2nfa r v), \<Delta>' (reg2nfa r v)) q w x}"
+      assume a3:"q \<in> \<I> (reg2nfa r v)"
+      assume a4:" xa \<in> \<F> (reg2nfa r v)"
+      assume a5:"LTS_is_reachable (\<Delta> (reg2nfa r v), \<Delta>' (reg2nfa r v)) q x xa"
+      show "\<exists>q''. (q'' = \<epsilon> \<or> q'' = r \<or> ((Ques r), q'') \<in> snd (trans2Del1 r v)) \<and> LTS_is_reachable (fst (trans2Del1 r v), insert ((Ques r), \<epsilon>) (insert ((Ques r), r) (snd (trans2Del1 r v)))) q'' x \<epsilon>"
      sorry
     qed
     subgoal for x 
     proof -
-      assume a1:"sem_reg r v = {w. ∃q∈ℐ (reg2nfa r v). ∃x∈ℱ (reg2nfa r v). LTS_is_reachable (Δ (reg2nfa r v), Δ' (reg2nfa r v)) q w x}" 
-      assume a2:"LTS_is_reachable (fst (trans2Del1 r v), insert (r?, ε) (insert (r?, r) (snd (trans2Del1 r v)))) r? x ε"
-      assume a3:"x ≠ []" 
-      show "∃q∈ℐ (reg2nfa r v). ∃xa∈ℱ (reg2nfa r v). LTS_is_reachable (Δ (reg2nfa r v), Δ' (reg2nfa r v)) q x xa "
+      assume a1:"sem_reg r v = {w. \<exists>q\<in>\<I> (reg2nfa r v). \<exists>x\<in>\<F> (reg2nfa r v). LTS_is_reachable (\<Delta> (reg2nfa r v), \<Delta>' (reg2nfa r v)) q w x}" 
+      assume a2:"LTS_is_reachable (fst (trans2Del1 r v), insert (Ques r, \<epsilon>) (insert (Ques r, r) (snd (trans2Del1 r v)))) (Ques r) x \<epsilon>"
+      assume a3:"x \<noteq> []" 
+      show "\<exists>q\<in>\<I> (reg2nfa r v). \<exists>xa\<in>\<F> (reg2nfa r v). LTS_is_reachable (\<Delta> (reg2nfa r v), \<Delta>' (reg2nfa r v)) q x xa "
         sorry
     qed
     done
